passification cfg helper lemma

BoogieLang/Passification.thy
@@ -99,7 +99,8 @@ inductive expr_rel :: "passive_rel \<Rightarrow> passive_rel \<Rightarrow> vdecl
               expr_list_rel R R_old loc_vars (x#xs) (y#ys)"
 
 method expr_rel_tac uses R_def R_old_def LocVar_assms = 
-  (match conclusion in "expr_rel ?R ?R_old ?loc_vars (Var ?x1) ?e2" \<Rightarrow> \<open>rule Var_Rel, solves \<open>simp add: R_def\<close>\<close> \<bar>
+  (match conclusion in "expr_rel ?R ?R_old ?loc_vars (Var ?x1) (Var ?x2)" \<Rightarrow> \<open>rule Var_Rel, solves \<open>simp add: R_def\<close>\<close> \<bar>
+                       "expr_rel ?R ?R_old ?loc_vars (Var ?x1) (Lit ?l)" \<Rightarrow> \<open>rule Var_Const_Rel, solves \<open>simp add: R_def\<close>\<close>  \<bar>
                        "expr_rel ?R ?R_old ?loc_vars (Old (Var ?x1)) ?e2" \<Rightarrow> 
                                \<open>rule OldGlobalVar_Rel, solves \<open>simp add: R_old_def\<close>  |
                                 rule OldLocalVar_Rel, solves \<open>simp add: LocVar_assms\<close>\<close> \<bar>
@@ -110,19 +111,20 @@ method expr_rel_tac uses R_def R_old_def LocVar_assms =
                        "_" \<Rightarrow> fail)+
 
 
-
-(* don't need to explicitly prove that constant has the declared type of the variable, since no 
-corresponding variable is constrained in the passive program *)
-definition rel_const_correct :: "var_context \<Rightarrow> passive_rel \<Rightarrow> 'a nstate \<Rightarrow> bool"
-  where "rel_const_correct \<Lambda> R ns = 
+definition rel_const_correct :: "var_context \<Rightarrow> rtype_env \<Rightarrow> passive_rel \<Rightarrow> 'a nstate \<Rightarrow> bool"
+  where "rel_const_correct \<Lambda> \<Omega> R ns = 
            (\<forall> x l. R x = Some (Inr l) \<longrightarrow>
-            ( lookup_var \<Lambda> ns x = Some (LitV l) ))"
+            (lookup_var \<Lambda> ns x = Some (LitV l) \<and> (\<exists> \<tau>. lookup_var_ty \<Lambda> x = Some \<tau> \<and> (TPrim (type_of_lit l)) = instantiate \<Omega> \<tau>)))"
+
+definition rel_const_correct_value :: "var_context \<Rightarrow> passive_rel \<Rightarrow> 'a nstate \<Rightarrow> bool"
+  where "rel_const_correct_value \<Lambda> R ns = 
+           (\<forall> x l. R x = Some (Inr l) \<longrightarrow> (lookup_var \<Lambda> ns x = Some (LitV l)))"
 
 definition rel_well_typed :: "'a absval_ty_fun \<Rightarrow> var_context \<Rightarrow> rtype_env \<Rightarrow> passive_rel \<Rightarrow> 'a nstate \<Rightarrow> bool"
   where "rel_well_typed A \<Lambda> \<Omega> R ns = (
            (\<forall> x y. R x = Some (Inl y) \<longrightarrow> 
              (\<exists>v \<tau>. lookup_var \<Lambda> ns x = Some v \<and> lookup_var_ty \<Lambda> x = Some \<tau> \<and> type_of_val A v = instantiate \<Omega> \<tau>)) \<and>
-           (rel_const_correct \<Lambda> R ns))"
+           (rel_const_correct \<Lambda> \<Omega> R ns))"
 
 lemma rel_well_typed_update: 
   assumes "rel_well_typed A \<Lambda> \<Omega> R ns" and "lookup_var_ty \<Lambda> x = Some \<tau>" and "type_of_val A v = instantiate \<Omega> \<tau>"
@@ -132,7 +134,7 @@ lemma rel_well_typed_update:
   by simp
 
 lemma rel_well_typed_update_const:
-  assumes "rel_well_typed A \<Lambda> \<Omega> R ns"
+  assumes "rel_well_typed A \<Lambda> \<Omega> R ns" and "lookup_var_ty \<Lambda> x = Some \<tau>" and "TPrim (type_of_lit l) = instantiate \<Omega> \<tau>"
   shows "rel_well_typed A \<Lambda> \<Omega> (R(x \<mapsto> Inr l)) (update_var \<Lambda> ns x (LitV l))"
   using assms
   unfolding rel_well_typed_def rel_const_correct_def
@@ -155,6 +157,28 @@ definition nstate_rel_states :: "var_context \<Rightarrow> var_context \<Rightar
 definition nstate_old_rel_states :: "var_context \<Rightarrow> var_context \<Rightarrow> passive_rel \<Rightarrow> 'a nstate \<Rightarrow> 'a nstate set \<Rightarrow> bool"
   where "nstate_old_rel_states \<Lambda> \<Lambda>' R ns U \<equiv> \<forall>u \<in> U. nstate_old_rel \<Lambda> \<Lambda>' R ns u"
 
+lemma nstate_rel_update: "nstate_rel \<Lambda> \<Lambda>' R ns1 ns2 \<Longrightarrow> lookup_var \<Lambda>' ns2 x' = Some v \<Longrightarrow> nstate_rel \<Lambda> \<Lambda>' (R(x \<mapsto> Inl x')) (update_var \<Lambda> ns1 x v) ns2"
+  unfolding nstate_rel_def
+  by (simp add: update_var_binder_same)
+
+lemma nstate_rel_update_2: 
+  assumes "nstate_rel \<Lambda> \<Lambda>' R ns1 ns2" and 
+          "R x' = Some (Inl x'')" and 
+          "lookup_var \<Lambda> ns1 x' = Some v"
+  shows    "nstate_rel \<Lambda> \<Lambda>' (R(x \<mapsto> Inl x'')) (update_var \<Lambda> ns1 x v) ns2"
+  using assms
+  unfolding nstate_rel_def
+  by (simp add: update_var_binder_same)
+
+lemma nstate_rel_states_update_2: 
+  assumes "nstate_rel_states \<Lambda> \<Lambda>' R ns1 U" and 
+          "R x' = Some (Inl x'')" and 
+          "lookup_var \<Lambda> ns1 x' = Some v"
+  shows    "nstate_rel_states \<Lambda> \<Lambda>' (R(x \<mapsto> Inl x'')) (update_var \<Lambda> ns1 x v) U"
+  using assms
+  unfolding nstate_rel_states_def
+  by (simp add: nstate_rel_update_2)
+  
 lemma nstate_rel_update_const: "nstate_rel \<Lambda> \<Lambda>' R ns1 ns2 \<Longrightarrow> nstate_rel \<Lambda> \<Lambda>' (R(x \<mapsto> Inr l)) (update_var \<Lambda> ns1 x v) ns2"
   unfolding nstate_rel_def
   by (simp add: update_var_binder_same)
@@ -231,6 +255,19 @@ next
   from Srel show "binder_state ns1 = binder_state ns2" by (simp add: nstate_rel_def)
 qed
 
+lemma update_rel_nstate_same_state_const:
+  assumes Srel: "nstate_rel \<Lambda> \<Lambda>' R ns1 ns2" and Lookup1:"lookup_var \<Lambda> ns1 x = Some (LitV l)" and Lookup2:"lookup_var \<Lambda>' ns2 x2 = Some (LitV l)"
+  shows "nstate_rel \<Lambda> \<Lambda>' (R(x \<mapsto> (Inl x2))) ns1 ns2"
+proof (unfold nstate_rel_def, rule+)
+  fix arg y
+  assume "(R(x \<mapsto> (Inl x2))) arg = Some (Inl y)"
+  thus "lookup_var \<Lambda> ns1 arg = lookup_var \<Lambda>' ns2 y"
+   using Srel Lookup1 Lookup2
+   by (metis (no_types, lifting) map_upd_Some_unfold nstate_rel_def sum.inject(1))
+next
+  from Srel show "binder_state ns1 = binder_state ns2" by (simp add: nstate_rel_def)
+qed
+
 lemma binder_update_nstate_rel: "nstate_rel \<Lambda> \<Lambda>' R ns1 ns2 \<Longrightarrow> (\<And>v. nstate_rel \<Lambda> \<Lambda>' R (full_ext_env ns1 v) (full_ext_env ns2 v))"
   unfolding nstate_rel_def
   apply (simp only: lookup_full_ext_env_same)
@@ -241,9 +278,13 @@ lemma binder_update_nstate_old_rel: "nstate_old_rel \<Lambda> \<Lambda>' R ns1 n
   apply (simp only: lookup_full_ext_env_same)
   by (simp add: binder_full_ext_env_same)
 
-lemma binder_update_rel_const: "rel_const_correct \<Lambda> R ns \<Longrightarrow> (\<And>v. rel_const_correct \<Lambda> R (full_ext_env ns v))"
+lemma binder_update_rel_const: "rel_const_correct \<Lambda> \<Omega> R ns \<Longrightarrow> (\<And>v. rel_const_correct \<Lambda> \<Omega> R (full_ext_env ns v))"
   unfolding rel_const_correct_def
   by (simp only: lookup_full_ext_env_same) auto  
+
+lemma binder_update_rel_const_value: "rel_const_correct_value \<Lambda> R ns \<Longrightarrow> (\<And>v. rel_const_correct_value \<Lambda> R (full_ext_env ns v))"
+  unfolding rel_const_correct_value_def
+  by (simp only: lookup_full_ext_env_same) auto
 
 lemma old_global_var_red:
   assumes "A,\<Lambda>,\<Gamma>,\<Omega> \<turnstile> \<langle>Old (Var x),ns\<rangle> \<Down> v" and "map_of (snd \<Lambda>) x = None"
@@ -282,13 +323,13 @@ lemma old_local_var_red:
 
 lemma expr_rel_same:
   shows "expr_rel R R_old (snd \<Lambda>) e1 e2 \<Longrightarrow>
-         rel_const_correct \<Lambda> R ns1 \<Longrightarrow> 
+         rel_const_correct_value \<Lambda> R ns1 \<Longrightarrow> 
          nstate_rel \<Lambda> \<Lambda>' R ns1 ns2 \<Longrightarrow> 
          nstate_old_rel \<Lambda> \<Lambda>' R_old ns1 ns2 \<Longrightarrow>
          A,\<Lambda>,\<Gamma>,\<Omega> \<turnstile> \<langle>e1, ns1\<rangle> \<Down> v \<Longrightarrow> 
          A,\<Lambda>',\<Gamma>,\<Omega> \<turnstile> \<langle>e2, ns2\<rangle> \<Down> v" and
     "expr_list_rel R R_old (snd \<Lambda>) es1 es2 \<Longrightarrow>
-     rel_const_correct \<Lambda> R ns1 \<Longrightarrow> 
+     rel_const_correct_value \<Lambda> R ns1 \<Longrightarrow> 
      nstate_rel \<Lambda> \<Lambda>' R ns1 ns2 \<Longrightarrow> 
      nstate_old_rel \<Lambda> \<Lambda>' R_old ns1 ns2 \<Longrightarrow>
      A,\<Lambda>,\<Gamma>,\<Omega> \<turnstile> \<langle>es1, ns1\<rangle> [\<Down>] vs \<Longrightarrow> 
@@ -313,7 +354,7 @@ next
   thus ?case  by (auto intro: red_expr_red_exprs.intros simp: nstate_rel_def)
 next
   case (Var_Const_Rel x1 l)
-  then show ?case by (auto intro: red_expr_red_exprs.intros simp: rel_const_correct_def)
+  then show ?case by (auto intro: red_expr_red_exprs.intros simp: rel_const_correct_value_def)
 next
   case (BVar_Rel x1 x2)
   thus ?case 
@@ -334,7 +375,7 @@ next
   case (Forall_Rel e1 e2 ty)
   hence RelExt:"\<And>v. nstate_rel \<Lambda> \<Lambda>' R (full_ext_env ns1 v) (full_ext_env ns2 v)" using binder_update_nstate_rel by blast
   from Forall_Rel have RelOldExt: "\<And>v. nstate_old_rel \<Lambda> \<Lambda>' R_old (full_ext_env ns1 v) (full_ext_env ns2 v)" using binder_update_nstate_old_rel by blast 
-  from Forall_Rel have RelWtExt:"\<And>v. rel_const_correct \<Lambda> R (full_ext_env ns1 v)" using binder_update_rel_const by blast   
+  from Forall_Rel have RelWtExt:"\<And>v. rel_const_correct_value \<Lambda> R (full_ext_env ns1 v)" using binder_update_rel_const_value by blast   
   from \<open>A,\<Lambda>,\<Gamma>,\<Omega> \<turnstile> \<langle>Forall ty e1,ns1\<rangle> \<Down> v\<close>     
   show ?case
     by (cases; blast intro: red_expr_red_exprs.intros dest:Forall_Rel.IH(2)[OF RelWtExt RelExt RelOldExt])
@@ -342,7 +383,7 @@ next
   case (Exists_Rel e1 e2 ty)
   hence RelExt:"\<And>v. nstate_rel \<Lambda> \<Lambda>' R (full_ext_env ns1 v) (full_ext_env ns2 v)" using binder_update_nstate_rel by blast
   from Exists_Rel have RelOldExt: "\<And>v. nstate_old_rel \<Lambda> \<Lambda>' R_old (full_ext_env ns1 v) (full_ext_env ns2 v)" using binder_update_nstate_old_rel by blast 
-  from Exists_Rel have RelWtExt:"\<And>v. rel_const_correct \<Lambda> R (full_ext_env ns1 v)" using binder_update_rel_const by blast 
+  from Exists_Rel have RelWtExt:"\<And>v. rel_const_correct_value \<Lambda> R (full_ext_env ns1 v)" using binder_update_rel_const_value by blast   
   from \<open>A,\<Lambda>,\<Gamma>,\<Omega> \<turnstile> \<langle>Exists ty e1,ns1\<rangle> \<Down> v\<close>
   show ?case
     by (cases; blast intro: red_expr_red_exprs.intros dest:Exists_Rel.IH(2)[OF RelWtExt RelExt RelOldExt])
@@ -350,12 +391,12 @@ next
   case (ForallT_Rel e1 e2)
   from \<open>A,\<Lambda>,\<Gamma>,\<Omega> \<turnstile> \<langle>ForallT e1,ns1\<rangle> \<Down> v\<close>
   show ?case
-    by cases (auto intro: red_expr_red_exprs.intros dest: ForallT_Rel.IH(2)[OF \<open>rel_const_correct \<Lambda> R ns1\<close> \<open>nstate_rel \<Lambda> \<Lambda>' R ns1 ns2\<close> \<open>nstate_old_rel \<Lambda> \<Lambda>' R_old ns1 ns2\<close>])
+    by cases (auto intro: red_expr_red_exprs.intros dest:ForallT_Rel.IH(2)[OF \<open>rel_const_correct_value \<Lambda> R ns1\<close> \<open>nstate_rel \<Lambda> \<Lambda>' R ns1 ns2\<close> \<open>nstate_old_rel \<Lambda> \<Lambda>' R_old ns1 ns2\<close>])
 next
   case (ExistsT_Rel e1 e2)
   from \<open>A,\<Lambda>,\<Gamma>,\<Omega> \<turnstile> \<langle>ExistsT e1,ns1\<rangle> \<Down> v\<close>
   show ?case
-    by cases (auto intro: red_expr_red_exprs.intros dest: ExistsT_Rel.IH(2)[OF \<open>rel_const_correct \<Lambda> R ns1\<close> \<open>nstate_rel \<Lambda> \<Lambda>' R ns1 ns2\<close> \<open>nstate_old_rel \<Lambda> \<Lambda>' R_old ns1 ns2\<close>])
+    by cases (auto intro: red_expr_red_exprs.intros dest: ExistsT_Rel.IH(2)[OF \<open>rel_const_correct_value \<Lambda> R ns1\<close> \<open>nstate_rel \<Lambda> \<Lambda>' R ns1 ns2\<close> \<open>nstate_old_rel \<Lambda> \<Lambda>' R_old ns1 ns2\<close>])
 next
   case Nil_Rel
   then show ?case
@@ -366,14 +407,19 @@ next
     by (blast elim: cons_exp_elim2 intro: red_expr_red_exprs.intros)
 qed
 
+lemma rel_const_correct_to_value:"rel_const_correct \<Lambda> \<Omega> R ns1 \<Longrightarrow> rel_const_correct_value \<Lambda> R ns1"
+  unfolding rel_const_correct_def rel_const_correct_value_def
+  by simp
+
 lemma expr_rel_same_set:
   assumes "expr_rel R R_old (snd \<Lambda>) e1 e2" and 
           "A,\<Lambda>,\<Gamma>,\<Omega> \<turnstile> \<langle>e1, ns1\<rangle> \<Down> v" and 
-          "rel_const_correct \<Lambda> R ns1" and
+          "rel_const_correct \<Lambda> \<Omega> R ns1" and
           "nstate_rel_states \<Lambda> \<Lambda>' R ns1 U" and
           "nstate_old_rel_states \<Lambda> \<Lambda>' R_old ns1 U"
   shows "\<forall>u \<in> U. A,\<Lambda>',\<Gamma>,\<Omega> \<turnstile> \<langle>e2, u\<rangle> \<Down> v"
-  using assms expr_rel_same unfolding nstate_rel_states_def nstate_old_rel_states_def by blast
+  using assms expr_rel_same(1) unfolding nstate_rel_states_def nstate_old_rel_states_def   
+  by (metis rel_const_correct_to_value)
 
 fun varsInExpr :: "expr \<Rightarrow> vname set"
   where
@@ -540,12 +586,37 @@ proof (unfold nstate_rel_states_def, rule ballI)
     by simp
 qed
 
+lemma assume_sync_const_nstate_rel:
+  assumes "R x_orig = Some (Inr l)" and
+          Srel:"nstate_rel_states \<Lambda> \<Lambda>' R ns U" and 
+          Rel_wt: "rel_well_typed A \<Lambda> \<Omega> R ns"
+  shows "nstate_rel_states \<Lambda> \<Lambda>' (R(x_orig \<mapsto> (Inl x2))) ns {ns'. Normal ns' \<in> (set_red_cmd A M \<Lambda>' \<Gamma> \<Omega> (Assume ((Var x2) \<guillemotleft>Eq\<guillemotright> (Lit l))) U)}"
+ (is "nstate_rel_states \<Lambda> \<Lambda>' (R(x_orig \<mapsto> (Inl x2))) ns ?U'")
+proof (unfold nstate_rel_states_def, rule ballI)
+  have Apassive:"isPassive (Assume ((Var x2) \<guillemotleft>Eq\<guillemotright> (Lit l)))" by simp
+  fix u'
+  assume "u' \<in> ?U'"
+  hence "u' \<in> U" using passive_states_subset[OF Apassive] by blast
+  with Srel have "nstate_rel \<Lambda> \<Lambda>' R ns u'" by (simp add: nstate_rel_states_def)
+  have "A,\<Lambda>',\<Gamma>,\<Omega> \<turnstile> \<langle>Lit l, u'\<rangle> \<Down> (LitV l)" by (rule RedLit)
+  from \<open>u' \<in> ?U'\<close> have "A,\<Lambda>',\<Gamma>,\<Omega> \<turnstile> \<langle>Var x2, u'\<rangle> \<Down> (LitV l)" 
+   using  expr_eval_determ(1)[OF \<open>A,\<Lambda>',\<Gamma>,\<Omega> \<turnstile> \<langle>Lit l, u'\<rangle> \<Down> LitV l\<close>] assume_reduction_args by metis
+  hence LookupX2:"lookup_var \<Lambda>' u' x2 = Some (LitV l)" by auto
+  from Rel_wt and \<open>R x_orig = Some (Inr l)\<close> have LookupOrig:"lookup_var \<Lambda> ns x_orig = Some (LitV l)"
+    unfolding rel_well_typed_def rel_const_correct_def
+    by simp
+  thus "nstate_rel \<Lambda> \<Lambda>' (R(x_orig \<mapsto> (Inl x2))) ns u'"
+    using update_rel_nstate_same_state_const[OF \<open>nstate_rel \<Lambda> \<Lambda>' R ns u'\<close>] LookupOrig LookupX2    
+    by blast    
+qed
+
+
 lemma assume_assign_nstate_rel:
   assumes Erel:"expr_rel R R_old (snd \<Lambda>) e1 e2" and
           "A,\<Lambda>,\<Gamma>,\<Omega> \<turnstile> \<langle>e1, ns\<rangle> \<Down> v" and
           Rel:"nstate_rel_states \<Lambda> \<Lambda>' R ns U" and
           OldRel: "nstate_old_rel_states \<Lambda> \<Lambda>' R_old ns U" and
-          CRel:"rel_const_correct \<Lambda> R ns"
+          CRel:"rel_const_correct \<Lambda> \<Omega> R ns"
   shows   "nstate_rel_states 
                \<Lambda> \<Lambda>' (R(x_orig \<mapsto> (Inl x))) (update_var \<Lambda> ns x_orig v) {ns'. Normal ns' \<in> (set_red_cmd A M \<Lambda>' \<Gamma> \<Omega> (Assume ((Var x) \<guillemotleft>Eq\<guillemotright> e2)) U)}" 
  (is "nstate_rel_states \<Lambda> \<Lambda>' (R(x_orig \<mapsto> (Inl x))) (update_var \<Lambda> ns x_orig v) ?U'")
@@ -555,8 +626,9 @@ proof (unfold nstate_rel_states_def, rule ballI)
   assume "u' \<in> ?U'"
   hence "u' \<in> U" using passive_states_subset[OF Apassive] by blast
   with Rel have Rel2:"nstate_rel \<Lambda> \<Lambda>' R ns u'" by (simp add: nstate_rel_states_def)
-  from \<open>u' \<in> U\<close> and OldRel have OldRel2:"nstate_old_rel \<Lambda> \<Lambda>' R_old ns u'" by (simp add: nstate_old_rel_states_def)
-  have "A,\<Lambda>',\<Gamma>,\<Omega> \<turnstile> \<langle>e2, u'\<rangle> \<Down> v" using expr_rel_same(1)[OF Erel CRel Rel2 OldRel2 \<open>A,\<Lambda>,\<Gamma>,\<Omega> \<turnstile> \<langle>e1, ns\<rangle> \<Down> v\<close>] by simp
+  from \<open>u' \<in> U\<close> and OldRel have OldRel2:"nstate_old_rel \<Lambda> \<Lambda>' R_old ns u'" by (simp add: nstate_old_rel_states_def)  
+  have "A,\<Lambda>',\<Gamma>,\<Omega> \<turnstile> \<langle>e2, u'\<rangle> \<Down> v" using expr_rel_same(1)[OF Erel _ Rel2 OldRel2 \<open>A,\<Lambda>,\<Gamma>,\<Omega> \<turnstile> \<langle>e1, ns\<rangle> \<Down> v\<close>] using CRel
+    using rel_const_correct_to_value by blast
   from \<open>u' \<in> ?U'\<close> have "A,\<Lambda>',\<Gamma>,\<Omega> \<turnstile> \<langle>Var x, u'\<rangle> \<Down> v" 
      using  expr_eval_determ(1)[OF \<open>A,\<Lambda>',\<Gamma>,\<Omega> \<turnstile> \<langle>e2, u'\<rangle> \<Down> v\<close>] assume_reduction_args by metis
   hence "lookup_var \<Lambda>' u' x = Some v" by auto
@@ -573,11 +645,16 @@ lemma single_assign_reduce_2:
     (\<exists>v \<tau>. (lookup_var_ty \<Lambda> x = Some \<tau>) \<and> (A,\<Lambda>,\<Gamma>,\<Omega> \<turnstile> \<langle>e, n_s\<rangle> \<Down> v) \<and> type_of_val A v = instantiate \<Omega> \<tau>)"
   by (erule red_cmd.cases) auto
 
+lemma single_assign_reduce_lit:
+  "A,M,\<Lambda>,\<Gamma>,\<Omega> \<turnstile> \<langle>Assign x (Lit l), Normal n_s\<rangle> \<rightarrow> s' \<Longrightarrow>  \<exists>\<tau>. lookup_var_ty \<Lambda> x = Some \<tau> \<and> (TPrim (type_of_lit l)) = instantiate \<Omega> \<tau>"
+  by (erule red_cmd.cases) auto
+  
+
 lemma assume_rel_normal:
   assumes Ared:"A,\<Lambda>,\<Gamma>,\<Omega> \<turnstile> \<langle>e1, ns\<rangle> \<Down> (BoolV True)" and
           Srel:"nstate_rel_states \<Lambda> \<Lambda>' R ns U" and 
           OldRel: "nstate_old_rel_states \<Lambda> \<Lambda>' R_old ns U" and
-          Crel:"rel_const_correct \<Lambda> R ns" and
+          Crel:"rel_const_correct \<Lambda> \<Omega> R ns" and
           Erel:"expr_rel R R_old (snd \<Lambda>) e1 e2"
         shows "\<And>u. u \<in> U \<Longrightarrow> A,M,\<Lambda>',\<Gamma>,\<Omega> \<turnstile> \<langle>Assume e2, Normal u\<rangle> \<rightarrow> Normal u"
 proof -
@@ -585,7 +662,7 @@ proof -
   assume "u \<in> U"
   with Srel OldRel have "nstate_rel \<Lambda> \<Lambda>' R ns u" and "nstate_old_rel \<Lambda> \<Lambda>' R_old ns u"    
       by (auto simp:  nstate_rel_states_def nstate_old_rel_states_def)
-  with Ared Erel have "A,\<Lambda>',\<Gamma>,\<Omega> \<turnstile> \<langle>e2, u\<rangle> \<Down> (BoolV True)" using expr_rel_same Crel by blast
+  with Ared Erel have "A,\<Lambda>',\<Gamma>,\<Omega> \<turnstile> \<langle>e2, u\<rangle> \<Down> (BoolV True)" using expr_rel_same(1) Crel rel_const_correct_to_value by metis
   thus "A,M,\<Lambda>',\<Gamma>,\<Omega> \<turnstile> \<langle>Assume e2,Normal u\<rangle> \<rightarrow> Normal u" by (auto intro: RedAssumeOk)
 qed
 
@@ -593,7 +670,7 @@ lemma assume_rel_magic:
   assumes Ared:"A,\<Lambda>,\<Gamma>,\<Omega> \<turnstile> \<langle>e1, ns\<rangle> \<Down> (BoolV False)" and
           Srel:"nstate_rel_states \<Lambda> \<Lambda>' R ns U" and
           OldRel: "nstate_old_rel_states \<Lambda> \<Lambda>' R_old ns U" and
-          Crel:"rel_const_correct \<Lambda> R ns" and
+          Crel:"rel_const_correct \<Lambda> \<Omega> R ns" and
           Erel:"expr_rel R R_old (snd \<Lambda>) e1 e2"
   shows "\<And>u. u \<in> U \<Longrightarrow> A,M,\<Lambda>',\<Gamma>,\<Omega> \<turnstile> \<langle>Assume e2, Normal u\<rangle> \<rightarrow> Magic"
 proof -
@@ -601,7 +678,7 @@ proof -
   assume "u \<in> U"
   with Srel OldRel have "nstate_rel \<Lambda> \<Lambda>' R ns u" and "nstate_old_rel \<Lambda> \<Lambda>' R_old ns u"    
     by (auto simp:  nstate_rel_states_def nstate_old_rel_states_def)
-  with Ared Erel have "A,\<Lambda>',\<Gamma>,\<Omega> \<turnstile> \<langle>e2, u\<rangle> \<Down> (BoolV False)" using expr_rel_same Crel by blast
+  with Ared Erel have "A,\<Lambda>',\<Gamma>,\<Omega> \<turnstile> \<langle>e2, u\<rangle> \<Down> (BoolV False)" using expr_rel_same(1) Crel rel_const_correct_to_value by metis
   thus "A,M,\<Lambda>',\<Gamma>,\<Omega> \<turnstile> \<langle>Assume e2,Normal u\<rangle> \<rightarrow> Magic" by (auto intro: RedAssumeMagic)
 qed
 
@@ -609,7 +686,7 @@ lemma assert_rel_normal:
   assumes Ared:"A,\<Lambda>,\<Gamma>,\<Omega> \<turnstile> \<langle>e1, ns\<rangle> \<Down> (BoolV True)" and
           Srel:"nstate_rel_states \<Lambda> \<Lambda>' R ns U" and 
           OldRel: "nstate_old_rel_states \<Lambda> \<Lambda>' R_old ns U" and
-          Crel:"rel_const_correct \<Lambda> R ns" and
+          Crel:"rel_const_correct \<Lambda> \<Omega> R ns" and
           Erel:"expr_rel R R_old (snd \<Lambda>) e1 e2"
   shows "{ns'. Normal ns' \<in> (set_red_cmd A M \<Lambda>' \<Gamma> \<Omega> (Assert e2) U)} = U" (is "?U' = U")
 proof 
@@ -622,7 +699,7 @@ next
     assume "u \<in> U"
     with Srel OldRel have "nstate_rel \<Lambda> \<Lambda>' R ns u" and "nstate_old_rel \<Lambda> \<Lambda>' R_old ns u"    
       by (auto simp:  nstate_rel_states_def nstate_old_rel_states_def)
-    with Ared Erel have "A,\<Lambda>',\<Gamma>,\<Omega> \<turnstile> \<langle>e2, u\<rangle> \<Down> (BoolV True)" using expr_rel_same Crel by blast
+    with Ared Erel have "A,\<Lambda>',\<Gamma>,\<Omega> \<turnstile> \<langle>e2, u\<rangle> \<Down> (BoolV True)" using expr_rel_same(1) Crel rel_const_correct_to_value by metis
     with \<open>u \<in> U\<close> show "u \<in> ?U'"
       by (auto intro!: red_cmd.intros simp: set_red_cmd_def)
   qed
@@ -632,7 +709,7 @@ lemma assert_rel_normal_2:
   assumes Ared:"A,\<Lambda>,\<Gamma>,\<Omega> \<turnstile> \<langle>e1, ns\<rangle> \<Down> (BoolV True)" and
           Srel:"nstate_rel_states \<Lambda> \<Lambda>' R ns U" and
           OldRel: "nstate_old_rel_states \<Lambda> \<Lambda>' R_old ns U" and
-          Crel:"rel_const_correct \<Lambda> R ns" and
+          Crel:"rel_const_correct \<Lambda> \<Omega> R ns" and
           Erel:"expr_rel R R_old (snd \<Lambda>) e1 e2"
         shows "\<And>u. u \<in> U \<Longrightarrow> A,M,\<Lambda>',\<Gamma>,\<Omega> \<turnstile> \<langle>Assert e2, Normal u\<rangle> \<rightarrow> Normal u"
 proof -
@@ -640,7 +717,7 @@ proof -
   assume "u \<in> U"
   with Srel OldRel have "nstate_rel \<Lambda> \<Lambda>' R ns u" and "nstate_old_rel \<Lambda> \<Lambda>' R_old ns u"    
     by (auto simp:  nstate_rel_states_def nstate_old_rel_states_def)
-  with Ared Erel have "A,\<Lambda>',\<Gamma>,\<Omega> \<turnstile> \<langle>e2, u\<rangle> \<Down> (BoolV True)" using expr_rel_same Crel by blast
+  with Ared Erel have "A,\<Lambda>',\<Gamma>,\<Omega> \<turnstile> \<langle>e2, u\<rangle> \<Down> (BoolV True)" using expr_rel_same(1) Crel rel_const_correct_to_value by metis
   thus "A,M,\<Lambda>',\<Gamma>,\<Omega> \<turnstile> \<langle>Assert e2,Normal u\<rangle> \<rightarrow> Normal u" by (auto intro: RedAssertOk)
 qed
 
@@ -648,7 +725,7 @@ lemma assert_rel_failure:
   assumes Ared:"A,\<Lambda>,\<Gamma>,\<Omega> \<turnstile> \<langle>e1, ns\<rangle> \<Down> (BoolV False)" and
           Srel:"nstate_rel_states \<Lambda> \<Lambda>' R ns U" and
           OldRel: "nstate_old_rel_states \<Lambda> \<Lambda>' R_old ns U" and
-          Crel:"rel_const_correct \<Lambda> R ns" and
+          Crel:"rel_const_correct \<Lambda> \<Omega> R ns" and
           Erel:"expr_rel R R_old (snd \<Lambda>) e1 e2"
   shows "\<And>u. u \<in> U \<Longrightarrow> A,M,\<Lambda>',\<Gamma>,\<Omega> \<turnstile> \<langle>Assert e2, Normal u\<rangle> \<rightarrow> Failure"
 proof -
@@ -656,7 +733,7 @@ proof -
   assume "u \<in> U"
   with Srel OldRel have "nstate_rel \<Lambda> \<Lambda>' R ns u" and "nstate_old_rel \<Lambda> \<Lambda>' R_old ns u"    
       by (auto simp:  nstate_rel_states_def nstate_old_rel_states_def)
-  with Ared Erel have "A,\<Lambda>',\<Gamma>,\<Omega> \<turnstile> \<langle>e2, u\<rangle> \<Down> (BoolV False)" using expr_rel_same Crel by blast
+  with Ared Erel have "A,\<Lambda>',\<Gamma>,\<Omega> \<turnstile> \<langle>e2, u\<rangle> \<Down> (BoolV False)" using expr_rel_same(1) Crel rel_const_correct_to_value by metis
   thus "A,M,\<Lambda>',\<Gamma>,\<Omega> \<turnstile> \<langle>Assert e2,Normal u\<rangle> \<rightarrow> Failure" by (auto intro: RedAssertFail)
 qed
 
@@ -688,14 +765,14 @@ lemma havoc_non_empty:
 
 (* evaluation of U on cs is in relation with s' *)
 definition passive_sim 
-  where "passive_sim A M \<Lambda> \<Lambda>' \<Gamma> \<Omega> cs s' R U \<equiv> 
+  where "passive_sim A M \<Lambda> \<Lambda>' \<Gamma> \<Omega> cs s' R R_old U \<equiv> 
               (\<forall>u \<in> U. \<exists>su. (A,M,\<Lambda>',\<Gamma>,\<Omega> \<turnstile> \<langle>cs, Normal u\<rangle> [\<rightarrow>] su) \<and> 
                        (s' = Failure \<longrightarrow> su = Failure) \<and>
-                       (\<forall>ns'. s' = Normal ns' \<longrightarrow> (su = Normal u \<and> nstate_rel \<Lambda> \<Lambda>' R ns' u \<and> rel_well_typed A \<Lambda> \<Omega> R ns')))"
+                       (\<forall>ns'. s' = Normal ns' \<longrightarrow> (su = Normal u \<and> nstate_rel \<Lambda> \<Lambda>' R ns' u \<and> nstate_old_rel \<Lambda> \<Lambda>' R_old ns' u \<and> rel_well_typed A \<Lambda> \<Omega> R ns')))"
 
 
 inductive passive_cmds_rel :: "vdecls \<Rightarrow> passive_rel \<Rightarrow> vname list \<Rightarrow> passive_rel \<Rightarrow> (vname \<times> (vname + lit)) list \<Rightarrow> cmd list \<Rightarrow> cmd list \<Rightarrow> bool"
-  for loc_vars :: vdecls and R_old :: passive_rel
+  for loc_vars :: vdecls and R_old :: passive_rel 
   where 
     PAssignNormal: 
     "\<lbrakk> expr_rel R R_old loc_vars e1 e2; passive_cmds_rel loc_vars R_old W (R(x1 \<mapsto> (Inl x2))) Q cs1 cs2 \<rbrakk> \<Longrightarrow> 
@@ -703,6 +780,9 @@ inductive passive_cmds_rel :: "vdecls \<Rightarrow> passive_rel \<Rightarrow> vn
   | PConst:
     " \<lbrakk> passive_cmds_rel loc_vars R_old W (R(x1 \<mapsto> (Inr l))) Q cs1 cs2 \<rbrakk> \<Longrightarrow>
        passive_cmds_rel loc_vars R_old W R ((x1, (Inr l))#Q) ((Assign x1 (Lit l))#cs1) cs2"
+  | PConstVar:
+    " \<lbrakk> R x1' = Some (Inl x2'); passive_cmds_rel loc_vars R_old W (R(x1 \<mapsto> (Inl x2'))) Q cs1 cs2 \<rbrakk> \<Longrightarrow>
+       passive_cmds_rel loc_vars R_old W R ((x1, (Inl x2'))#Q) ((Assign x1 (Var x1'))#cs1) cs2"
   | PAssert: 
     "\<lbrakk> expr_rel R R_old loc_vars e1 e2; passive_cmds_rel loc_vars R_old W R Q cs1 cs2 \<rbrakk> \<Longrightarrow> 
         passive_cmds_rel loc_vars R_old W R Q ((Assert e1) # cs1) ((Assert e2) # cs2)"
@@ -711,22 +791,29 @@ inductive passive_cmds_rel :: "vdecls \<Rightarrow> passive_rel \<Rightarrow> vn
         passive_cmds_rel loc_vars R_old W R Q ((Assume e1) # cs1) ((Assume e2) # cs2)"
   | PHavoc: 
     "\<lbrakk> passive_cmds_rel loc_vars R_old W (R(x \<mapsto> (Inl x'))) Q cs1 cs2\<rbrakk> \<Longrightarrow> 
-       passive_cmds_rel loc_vars R_old (x'#W) R ((x,(Inl x'))#Q) ((Havoc x) # cs1) cs2"
+       passive_cmds_rel loc_vars R_old (x'#W) R ((x,(Inl x'))#Q) ((Havoc x) # cs1) cs2"  
   | PSync:       
     "\<lbrakk> R x = Some (Inl x1); passive_cmds_rel loc_vars R_old W (R(x \<mapsto> (Inl x2))) Q [] cs \<rbrakk> \<Longrightarrow>
        passive_cmds_rel loc_vars R_old (x2#W) R ((x,(Inl x2))#Q) [] ((Assume ( (Var x2) \<guillemotleft>Eq\<guillemotright> (Var x1))) # cs)"
+  | PSyncConst:
+    "\<lbrakk> R x = Some (Inr l); passive_cmds_rel loc_vars R_old W (R(x \<mapsto> (Inl x2))) Q [] cs \<rbrakk> \<Longrightarrow>
+       passive_cmds_rel loc_vars R_old (x2#W) R ((x,(Inl x2))#Q) [] ((Assume ( (Var x2) \<guillemotleft>Eq\<guillemotright> (Lit l))) # cs)"
   | PNil: "passive_cmds_rel loc_vars R_old [] R [] [] []"
 
 
-method passive_rel_tac uses R_def R_old_def LocVar_assms = 
+method passive_rel_tac_single uses R_def R_old_def LocVar_assms = 
   (match conclusion in                       
                        "passive_cmds_rel ?loc_vars ?R_old ?W ?R ?Q ((Assign ?x1 (Lit ?l))#?cs1) ?cs2" \<Rightarrow> \<open>rule PConst\<close> \<bar>
+                       "passive_cmds_rel ?loc_vars ?R_old ?W ?R ?Q ((Assign ?x1 (Var ?x1'))#?cs1) ?cs2" \<Rightarrow> \<open>rule PConstVar,solves \<open>simp add: R_def\<close>\<close> \<bar>
                        "passive_cmds_rel ?loc_vars ?R_old ?W ?R ?Q ((Havoc ?x1)#?cs1) ?cs2" \<Rightarrow> \<open>rule PHavoc\<close> \<bar>
                        "passive_cmds_rel ?loc_vars ?R_old ?W ?R ?Q [] []" \<Rightarrow> \<open>rule PNil\<close> \<bar>
-                       "passive_cmds_rel ?loc_vars ?R_old ?W ?R ?Q [] ?cs2" \<Rightarrow> \<open>rule PSync, solves \<open>simp add: R_def\<close>\<close>  \<bar>
+                       "passive_cmds_rel ?loc_vars ?R_old ?W ?R ?Q [] ?cs2" \<Rightarrow> \<open>(rule PSync | rule PSyncConst), solves \<open>simp add: R_def\<close>\<close>  \<bar>
                        "passive_cmds_rel ?loc_vars ?R_old ?W ?R ?Q ?cs1 ?cs2" \<Rightarrow>
                           \<open>rule, solves \<open>expr_rel_tac R_def: R_def R_old_def: R_old_def LocVar_assms: LocVar_assms\<close>\<close> \<bar>                 
-                       "_" \<Rightarrow> fail)+
+                       "_" \<Rightarrow> fail)
+
+method passive_rel_tac uses R_def R_old_def LocVar_assms = 
+  (passive_rel_tac_single R_def: R_def R_old_def: R_old_def LocVar_assms: LocVar_assms)+
 
 (* "semantic" block lemma *)
 (*
@@ -764,7 +851,7 @@ lemma passification_block_lemma_aux:
           "U0 \<noteq> {}" and
           "type_rel \<Lambda> \<Lambda>' Q" and
           "distinct W"
-        shows "\<exists> U1 \<subseteq> U0. U1 \<noteq> {} \<and> dependent A \<Lambda>' \<Omega> U1 (D0 \<union> (set W)) \<and> passive_sim A M \<Lambda> \<Lambda>' \<Gamma> \<Omega> cs2 s' (update_nstate_rel R Q) U1"
+        shows "\<exists> U1 \<subseteq> U0. U1 \<noteq> {} \<and> dependent A \<Lambda>' \<Omega> U1 (D0 \<union> (set W)) \<and> passive_sim A M \<Lambda> \<Lambda>' \<Gamma> \<Omega> cs2 s' (update_nstate_rel R Q) R_old U1"
   unfolding passive_sim_def
 (*
   shows "\<exists> U1 \<subseteq> U0. U1 \<noteq> {} \<and> dependent \<Lambda>' U1 (D0 \<union> (set W)) \<and>
@@ -774,11 +861,11 @@ lemma passification_block_lemma_aux:
   using assms
 proof (induction arbitrary: ns U0 D0)
 case (PAssignNormal R e1 e2 W x1 x2 Q cs1 cs2)  (* TODO: share proof with case PSync *)
-  hence "x2 \<notin> D0" and "rel_const_correct \<Lambda> R ns" by (auto simp: rel_well_typed_def)
+  hence "x2 \<notin> D0" and "rel_const_correct \<Lambda> \<Omega> R ns" by (auto simp: rel_well_typed_def)
   from \<open>A,M,\<Lambda>,\<Gamma>,\<Omega> \<turnstile> \<langle>Assign x1 e1 # cs1,Normal ns\<rangle> [\<rightarrow>] s'\<close> obtain v1 \<tau>
     where RedE1:"A,\<Lambda>,\<Gamma>,\<Omega> \<turnstile> \<langle>e1,ns\<rangle> \<Down> v1" and LookupX1:"lookup_var_ty \<Lambda> x1 = Some \<tau>" and 
                 TyV1:"type_of_val A v1 = instantiate \<Omega> \<tau>" by (meson RedCmdListCons_case single_assign_reduce_2)
-  with expr_rel_same_set[OF \<open>expr_rel R R_old (snd \<Lambda>) e1 e2\<close> _ \<open>rel_const_correct \<Lambda> R ns\<close> \<open>nstate_rel_states \<Lambda> \<Lambda>' R ns U0\<close> \<open>nstate_old_rel_states \<Lambda> \<Lambda>' R_old ns U0\<close>]
+  with expr_rel_same_set[OF \<open>expr_rel R R_old (snd \<Lambda>) e1 e2\<close> _ \<open>rel_const_correct \<Lambda> \<Omega> R ns\<close> \<open>nstate_rel_states \<Lambda> \<Lambda>' R ns U0\<close> \<open>nstate_old_rel_states \<Lambda> \<Lambda>' R_old ns U0\<close>]
   have RedE2:"\<forall>u\<in>U0. A, \<Lambda>',\<Gamma>,\<Omega> \<turnstile> \<langle>e2,u\<rangle> \<Down> v1" by blast  
   from LookupX1 have LookupX2:"lookup_var_ty \<Lambda>' x2 = Some \<tau>" using \<open>type_rel \<Lambda> \<Lambda>' ((x1, (Inl x2)) # Q)\<close> by (simp add: type_rel_def)
   let ?U1 = "(set_red_cmd A M \<Lambda>' \<Gamma> \<Omega> (Assume ((Var x2) \<guillemotleft>Eq\<guillemotright> e2)) U0)"
@@ -790,7 +877,7 @@ case (PAssignNormal R e1 e2 W x1 x2 Q cs1 cs2)  (* TODO: share proof with case P
   have U1Dep: "dependent A \<Lambda>' \<Omega> ?U1Normal (D0 \<union> {x2})" using \<open>x2 \<notin> D0\<close> \<open>dependent A \<Lambda>' \<Omega> U0 D0\<close> RedE2    
     by (blast dest:  assume_assign_dependent)
     have RelStates: "nstate_rel_states \<Lambda> \<Lambda>' (R(x1 \<mapsto> (Inl x2))) (update_var \<Lambda> ns x1 v1) ?U1Normal"
-      using \<open>nstate_rel_states \<Lambda> \<Lambda>' R ns U0\<close> \<open>nstate_old_rel_states \<Lambda> \<Lambda>' R_old ns U0\<close> \<open>expr_rel R R_old (snd \<Lambda>) e1 e2\<close> \<open>rel_const_correct \<Lambda> R ns\<close> RedE1
+      using \<open>nstate_rel_states \<Lambda> \<Lambda>' R ns U0\<close> \<open>nstate_old_rel_states \<Lambda> \<Lambda>' R_old ns U0\<close> \<open>expr_rel R R_old (snd \<Lambda>) e1 e2\<close> \<open>rel_const_correct \<Lambda> \<Omega> R ns\<close> RedE1
       by (blast dest: assume_assign_nstate_rel)
     have RelOldStates: "nstate_old_rel_states \<Lambda> \<Lambda>' R_old (update_var \<Lambda> ns x1 v1) ?U1Normal"
       using \<open>nstate_old_rel_states \<Lambda> \<Lambda>' R_old ns U0\<close> U1Sub nstate_old_rel_states_update nstate_old_rel_states_subset
@@ -809,7 +896,7 @@ case (PAssignNormal R e1 e2 W x1 x2 Q cs1 cs2)  (* TODO: share proof with case P
     U2Rel:"(\<forall>u\<in>U2.
          \<exists>su. (A,M,\<Lambda>',\<Gamma>,\<Omega> \<turnstile> \<langle>cs2,Normal u\<rangle> [\<rightarrow>] su) \<and>
               (s' = Failure \<longrightarrow> su = Failure) \<and> 
-              (\<forall>ns'. s' = Normal ns' \<longrightarrow> su = Normal u \<and> nstate_rel \<Lambda> \<Lambda>' (update_nstate_rel (R(x1 \<mapsto> (Inl x2))) Q) ns' u \<and> rel_well_typed A \<Lambda> \<Omega> (update_nstate_rel (R(x1 \<mapsto> (Inl x2))) Q) ns'))"
+              (\<forall>ns'. s' = Normal ns' \<longrightarrow> su = Normal u \<and> nstate_rel \<Lambda> \<Lambda>' (update_nstate_rel (R(x1 \<mapsto> (Inl x2))) Q) ns' u \<and> nstate_old_rel \<Lambda> \<Lambda>' R_old ns' u \<and> rel_well_typed A \<Lambda> \<Omega> (update_nstate_rel (R(x1 \<mapsto> (Inl x2))) Q) ns'))"
     by blast
   hence U2Sub':"U2 \<subseteq> U0" and  U2Dep':"dependent A \<Lambda>' \<Omega> U2 (D0 \<union> set (x2 # W))" and 
         RedAssume2:"\<And>u. u \<in> U2 \<Longrightarrow> A,M,\<Lambda>',\<Gamma>,\<Omega> \<turnstile> \<langle>Assume ((Var x2) \<guillemotleft>Eq\<guillemotright> e2),Normal u\<rangle> \<rightarrow> Normal u" using U1Sub RedAssume by auto
@@ -820,14 +907,16 @@ case (PAssignNormal R e1 e2 W x1 x2 Q cs1 cs2)  (* TODO: share proof with case P
 next
   case (PConst W R x1 l Q cs1 cs2)
   let ?ns' = "(update_var \<Lambda> ns x1 (LitV l))"
-  from \<open>A,M,\<Lambda>,\<Gamma>,\<Omega> \<turnstile> \<langle>Assign x1 (Lit l) # cs1,Normal ns\<rangle> [\<rightarrow>] s'\<close> have
-      RedCs1:\<open>A,M,\<Lambda>,\<Gamma>,\<Omega> \<turnstile> \<langle>cs1,Normal ?ns'\<rangle> [\<rightarrow>] s'\<close>       
-    by (metis RedCmdListCons_case single_assign_cases val_elim)
+  from \<open>A,M,\<Lambda>,\<Gamma>,\<Omega> \<turnstile> \<langle>Assign x1 (Lit l) # cs1,Normal ns\<rangle> [\<rightarrow>] s'\<close> obtain \<tau> where
+      RedCs1:\<open>A,M,\<Lambda>,\<Gamma>,\<Omega> \<turnstile> \<langle>cs1,Normal ?ns'\<rangle> [\<rightarrow>] s'\<close> and "lookup_var_ty \<Lambda> x1 = Some \<tau>" and
+       TypeLit:"TPrim (type_of_lit l) = instantiate \<Omega> \<tau>"
+    by (metis RedCmdListCons_case single_assign_cases single_assign_reduce_lit val_elim)
+    
   from \<open>nstate_rel_states \<Lambda> \<Lambda>' R ns U0\<close> have RelStates:"nstate_rel_states \<Lambda> \<Lambda>' (R(x1 \<mapsto> Inr l)) ?ns' U0" by (simp add: nstate_rel_states_update_const)
   from \<open>nstate_old_rel_states \<Lambda> \<Lambda>' R_old ns U0\<close> have RelOldStates:"nstate_old_rel_states \<Lambda> \<Lambda>' R_old ?ns' U0" by (simp add: nstate_old_rel_states_update)  
-  from \<open>rel_well_typed A \<Lambda> \<Omega> R ns\<close> have Rel_wt:"rel_well_typed A \<Lambda> \<Omega> (R(x1 \<mapsto> Inr l)) ?ns'" by (simp add: rel_well_typed_update_const)
+  from \<open>rel_well_typed A \<Lambda> \<Omega> R ns\<close> have Rel_wt:"rel_well_typed A \<Lambda> \<Omega> (R(x1 \<mapsto> Inr l)) ?ns'"
+       using \<open>lookup_var_ty \<Lambda> x1 = Some \<tau>\<close> TypeLit by (simp add: rel_well_typed_update_const)
   from \<open>type_rel \<Lambda> \<Lambda>' ((x1, Inr l) # Q)\<close> have QTyRel:"type_rel \<Lambda> \<Lambda>' Q" by (simp add: type_rel_def)
-
   from PConst.IH[OF RedCs1 \<open>dependent A \<Lambda>' \<Omega> U0 D0\<close> RelStates RelOldStates Rel_wt _ _ QTyRel] obtain U1 where
     "U1 \<subseteq> U0" and "U1 \<noteq> {}" and "dependent A \<Lambda>' \<Omega> U1 (D0 \<union> set W)" and
     "(\<forall>u\<in>U1.
@@ -835,13 +924,38 @@ next
               (s' = Failure \<longrightarrow> su = Failure) \<and>
               (\<forall>ns'. s' = Normal ns' \<longrightarrow>
                      su = Normal u \<and>
-                     nstate_rel \<Lambda> \<Lambda>' (update_nstate_rel (R(x1 \<mapsto> Inr l)) Q) ns' u \<and> rel_well_typed A \<Lambda> \<Omega> (update_nstate_rel (R(x1 \<mapsto> Inr l)) Q) ns'))"
+                     nstate_rel \<Lambda> \<Lambda>' (update_nstate_rel (R(x1 \<mapsto> Inr l)) Q) ns' u \<and> nstate_old_rel \<Lambda> \<Lambda>' R_old ns' u \<and> rel_well_typed A \<Lambda> \<Omega> (update_nstate_rel (R(x1 \<mapsto> Inr l)) Q) ns'))"
     using PConst by blast    
   then show ?case using update_nstate_rel_cons
     by metis
 next
+  case (PConstVar R x1' x2' W x1 Q cs1 cs2)
+  from \<open>A,M,\<Lambda>,\<Gamma>,\<Omega> \<turnstile> \<langle>Assign x1 (Var x1') # cs1,Normal ns\<rangle> [\<rightarrow>] s'\<close> obtain v \<tau>
+    where LookupX1':"lookup_var \<Lambda> ns x1' = Some v" and RedCs1:"A,M,\<Lambda>,\<Gamma>,\<Omega> \<turnstile> \<langle>cs1,Normal (update_var \<Lambda> ns x1 v)\<rangle> [\<rightarrow>] s'" and
+         LookupTyX1:"lookup_var_ty \<Lambda> x1 = Some \<tau>" and TyV:"type_of_val A v = instantiate \<Omega> \<tau>"
+    by (metis RedCmdListCons_case RedVar_case option.sel single_assign_cases single_assign_reduce_2)
+  let ?ns' = "(update_var \<Lambda> ns x1 v)"
+  from LookupX1' have RelStates:"nstate_rel_states \<Lambda> \<Lambda>' (R(x1 \<mapsto> Inl x2')) ?ns' U0"
+    using \<open>nstate_rel_states \<Lambda> \<Lambda>' R ns U0\<close> \<open>R x1' = Some (Inl x2')\<close>    
+    by (simp add: nstate_rel_states_update_2)
+  from \<open>nstate_old_rel_states \<Lambda> \<Lambda>' R_old ns U0\<close> have RelOldStates:"nstate_old_rel_states \<Lambda> \<Lambda>' R_old ?ns' U0" by (simp add: nstate_old_rel_states_update)  
+  from \<open>rel_well_typed A \<Lambda> \<Omega> R ns\<close> have Rel_wt:"rel_well_typed A \<Lambda> \<Omega> (R(x1 \<mapsto> Inl x2')) ?ns'" using LookupTyX1 TyV rel_well_typed_update by blast
+  from \<open>type_rel \<Lambda> \<Lambda>' ((x1, Inl x2') # Q)\<close> have QTyRel:"type_rel \<Lambda> \<Lambda>' Q" by (simp add: type_rel_def)
+
+  from PConstVar.IH[OF RedCs1 \<open>dependent A \<Lambda>' \<Omega> U0 D0\<close> RelStates RelOldStates Rel_wt _ _ QTyRel] obtain U1 where
+    "U1 \<subseteq> U0" and "U1 \<noteq> {}" and "dependent A \<Lambda>' \<Omega> U1 (D0 \<union> set W)" and
+    "(\<forall>u\<in>U1.
+         \<exists>su. (A,M,\<Lambda>',\<Gamma>,\<Omega> \<turnstile> \<langle>cs2,Normal u\<rangle> [\<rightarrow>] su) \<and>
+              (s' = Failure \<longrightarrow> su = Failure) \<and>
+              (\<forall>ns'. s' = Normal ns' \<longrightarrow>
+                     su = Normal u \<and>
+                     nstate_rel \<Lambda> \<Lambda>' (update_nstate_rel (R(x1 \<mapsto> Inl x2')) Q) ns' u \<and> nstate_old_rel \<Lambda> \<Lambda>' R_old ns' u \<and> rel_well_typed A \<Lambda> \<Omega> (update_nstate_rel (R(x1 \<mapsto> Inl x2')) Q) ns'))"
+    using PConstVar by blast 
+  then show ?case using update_nstate_rel_cons
+    by metis
+next
   case (PAssert R e1 e2 W Q cs1 cs2)
-  hence "rel_const_correct \<Lambda> R ns" by (simp add: rel_well_typed_def)
+  hence "rel_const_correct \<Lambda> \<Omega> R ns" by (simp add: rel_well_typed_def)
   from \<open>A,M,\<Lambda>,\<Gamma>,\<Omega> \<turnstile> \<langle>Assert e1 # cs1,Normal ns\<rangle> [\<rightarrow>] s'\<close> obtain s'' where 
     RedAssert:"A,M,\<Lambda>,\<Gamma>,\<Omega> \<turnstile> \<langle>Assert e1,Normal ns\<rangle> \<rightarrow> s''" and
     RedCs1:"A,M,\<Lambda>,\<Gamma>,\<Omega> \<turnstile> \<langle>cs1, s''\<rangle> [\<rightarrow>] s'" 
@@ -851,14 +965,14 @@ next
     case RedAssertOk
     hence RedE2:"\<And>u. u\<in>U0 \<Longrightarrow> A,M,\<Lambda>',\<Gamma>,\<Omega> \<turnstile> \<langle>Assert e2,Normal u\<rangle> \<rightarrow> Normal u"
       using assert_rel_normal_2 \<open>nstate_rel_states \<Lambda> \<Lambda>' R ns U0\<close>  \<open>nstate_old_rel_states \<Lambda> \<Lambda>' R_old ns U0\<close> 
-           \<open>expr_rel R R_old (snd \<Lambda>) e1 e2\<close> \<open>rel_const_correct \<Lambda> R ns\<close> by blast
+           \<open>expr_rel R R_old (snd \<Lambda>) e1 e2\<close> \<open>rel_const_correct \<Lambda> \<Omega> R ns\<close> by blast
     from \<open>s'' = Normal ns\<close> RedCs1 have RedCs1Normal:"A,M,\<Lambda>,\<Gamma>,\<Omega> \<turnstile> \<langle>cs1, Normal ns\<rangle> [\<rightarrow>] s'" by simp
     from PAssert.IH[OF RedCs1Normal \<open>dependent A \<Lambda>' \<Omega> U0 D0\<close>] obtain U1 
       where U1Sub: "U1 \<subseteq> U0" and "U1 \<noteq> {}" and U1Dep:"dependent A \<Lambda>' \<Omega> U1 (D0 \<union> set W)" and
        U1Rel:"(\<forall>u\<in>U1.
            \<exists>su. (A,M,\<Lambda>',\<Gamma>,\<Omega> \<turnstile> \<langle>cs2,Normal u\<rangle> [\<rightarrow>] su) \<and>
                 (s' = Failure \<longrightarrow> su = Failure) \<and>
-                (\<forall>ns'. s' = Normal ns' \<longrightarrow> su = Normal u \<and> nstate_rel \<Lambda> \<Lambda>' (update_nstate_rel R Q) ns' u \<and> rel_well_typed A \<Lambda> \<Omega> (update_nstate_rel R Q) ns') )"
+                (\<forall>ns'. s' = Normal ns' \<longrightarrow> su = Normal u \<and> nstate_rel \<Lambda> \<Lambda>' (update_nstate_rel R Q) ns' u \<and> nstate_old_rel \<Lambda> \<Lambda>' R_old ns' u \<and> rel_well_typed A \<Lambda> \<Omega> (update_nstate_rel R Q) ns') )"
       using PAssert.prems by auto
     show ?thesis 
       apply (rule exI, intro conjI)
@@ -871,7 +985,7 @@ next
     case RedAssertFail
     hence RedE2:"\<And>u. u\<in>U0 \<Longrightarrow> A,M,\<Lambda>',\<Gamma>,\<Omega> \<turnstile> \<langle>Assert e2,Normal u\<rangle> \<rightarrow> Failure" 
       using assert_rel_failure \<open>nstate_rel_states \<Lambda> \<Lambda>' R ns U0\<close> \<open>nstate_old_rel_states \<Lambda> \<Lambda>' R_old ns U0\<close>
-            \<open>expr_rel R R_old (snd \<Lambda>) e1 e2\<close> \<open>rel_const_correct \<Lambda> R ns\<close> by blast
+            \<open>expr_rel R R_old (snd \<Lambda>) e1 e2\<close> \<open>rel_const_correct \<Lambda> \<Omega> R ns\<close> by blast
     from  \<open>s'' = Failure\<close> have "s' = Failure" using RedCs1
       by (simp add: failure_stays_cmd_list)
     show ?thesis
@@ -883,7 +997,7 @@ next
   qed
 next
   case (PAssumeNormal R e1 e2 W Q cs1 cs2)
-  hence "rel_const_correct \<Lambda> R ns" by (simp add: rel_well_typed_def)
+  hence "rel_const_correct \<Lambda> \<Omega> R ns" by (simp add: rel_well_typed_def)
   from \<open>A,M,\<Lambda>,\<Gamma>,\<Omega> \<turnstile> \<langle>Assume e1 # cs1,Normal ns\<rangle> [\<rightarrow>] s'\<close> obtain s'' where 
     RedAssume:"A,M,\<Lambda>,\<Gamma>,\<Omega> \<turnstile> \<langle>Assume e1,Normal ns\<rangle> \<rightarrow> s''" and
     RedCs1:"A,M,\<Lambda>,\<Gamma>,\<Omega> \<turnstile> \<langle>cs1, s''\<rangle> [\<rightarrow>] s'" 
@@ -893,14 +1007,14 @@ next
     case RedAssumeOk
     hence RedE2:"\<And>u. u\<in>U0 \<Longrightarrow> A,M,\<Lambda>',\<Gamma>,\<Omega> \<turnstile> \<langle>Assume e2,Normal u\<rangle> \<rightarrow> Normal u"
       using assume_rel_normal \<open>nstate_rel_states \<Lambda> \<Lambda>' R ns U0\<close> \<open>nstate_old_rel_states \<Lambda> \<Lambda>' R_old ns U0\<close>
-            \<open>expr_rel R R_old (snd \<Lambda>) e1 e2\<close> \<open>rel_const_correct \<Lambda> R ns\<close> by blast
+            \<open>expr_rel R R_old (snd \<Lambda>) e1 e2\<close> \<open>rel_const_correct \<Lambda> \<Omega> R ns\<close> by blast
     from \<open>s'' = Normal ns\<close> RedCs1 have RedCs1Normal:"A,M,\<Lambda>,\<Gamma>,\<Omega> \<turnstile> \<langle>cs1, Normal ns\<rangle> [\<rightarrow>] s'" by simp
     from PAssumeNormal.IH[OF RedCs1Normal \<open>dependent A \<Lambda>' \<Omega> U0 D0\<close>] obtain U1 
       where U1Sub: "U1 \<subseteq> U0" and "U1 \<noteq> {}" and U1Dep:"dependent A \<Lambda>' \<Omega> U1 (D0 \<union> set W)" and
        U1Rel:"(\<forall>u\<in>U1.
            \<exists>su. (A,M,\<Lambda>',\<Gamma>,\<Omega> \<turnstile> \<langle>cs2,Normal u\<rangle> [\<rightarrow>] su) \<and>
                 (s' = Failure \<longrightarrow> su = Failure) \<and>
-                (\<forall>ns'. s' = Normal ns' \<longrightarrow> su = Normal u \<and> nstate_rel \<Lambda> \<Lambda>' (update_nstate_rel R Q) ns' u \<and> rel_well_typed A \<Lambda> \<Omega> (update_nstate_rel R Q) ns'))"
+                (\<forall>ns'. s' = Normal ns' \<longrightarrow> su = Normal u \<and> nstate_rel \<Lambda> \<Lambda>' (update_nstate_rel R Q) ns' u \<and> nstate_old_rel \<Lambda> \<Lambda>' R_old ns' u \<and> rel_well_typed A \<Lambda> \<Omega> (update_nstate_rel R Q) ns'))"
       using PAssumeNormal.prems by auto
     show ?thesis 
       apply (rule exI, intro conjI)
@@ -913,7 +1027,7 @@ next
     case RedAssumeMagic
     hence  RedE2:"\<And>u. u\<in>U0 \<Longrightarrow> A,M,\<Lambda>',\<Gamma>,\<Omega> \<turnstile> \<langle>Assume e2,Normal u\<rangle> \<rightarrow> Magic"
       using assume_rel_magic \<open>nstate_rel_states \<Lambda> \<Lambda>' R ns U0\<close> \<open>nstate_old_rel_states \<Lambda> \<Lambda>' R_old ns U0\<close>
-            \<open>expr_rel R R_old (snd \<Lambda>) e1 e2\<close> \<open>rel_const_correct \<Lambda> R ns\<close> by blast
+            \<open>expr_rel R R_old (snd \<Lambda>) e1 e2\<close> \<open>rel_const_correct \<Lambda> \<Omega> R ns\<close> by blast
     from \<open>s'' = Magic\<close> have "s' = Magic" using RedCs1
       by (simp add: magic_stays_cmd_list) 
     show ?thesis 
@@ -951,7 +1065,7 @@ next
        "(\<forall>u\<in>U2.
          \<exists>su. (A,M,\<Lambda>',\<Gamma>,\<Omega> \<turnstile> \<langle>cs2,Normal u\<rangle> [\<rightarrow>] su) \<and>
               (s' = Failure \<longrightarrow> su = Failure) \<and>
-              (\<forall>ns'. s' = Normal ns' \<longrightarrow> su = Normal u \<and> nstate_rel \<Lambda> \<Lambda>' (update_nstate_rel (R(x \<mapsto> Inl x')) Q) ns' u \<and> rel_well_typed A \<Lambda> \<Omega> (update_nstate_rel (R(x \<mapsto> Inl x')) Q) ns'))"
+              (\<forall>ns'. s' = Normal ns' \<longrightarrow> su = Normal u \<and> nstate_rel \<Lambda> \<Lambda>' (update_nstate_rel (R(x \<mapsto> Inl x')) Q) ns' u \<and> nstate_old_rel \<Lambda> \<Lambda>' R_old ns' u \<and> rel_well_typed A \<Lambda> \<Omega> (update_nstate_rel (R(x \<mapsto> Inl x')) Q) ns'))"
     by blast 
   thus ?case    
     apply (simp)
@@ -975,7 +1089,7 @@ next
     using \<open>nstate_rel_states \<Lambda> \<Lambda>' R ns U0\<close> \<open>R x = Some (Inl x1)\<close> \<open>rel_well_typed A \<Lambda> \<Omega> R ns\<close> by (fastforce dest: lookup_nstates_rel intro: RedVar)
   from LookupTy have "lookup_var_ty \<Lambda>' x2 = Some \<tau>" using \<open>type_rel \<Lambda> \<Lambda>' ((x, Inl x2) # Q)\<close> by (simp add: type_rel_def)
   hence U1NonEmpty: "?U1Normal \<noteq> {}" using RedX1 \<open>U0 \<noteq> {}\<close> \<open>dependent A \<Lambda>' \<Omega> U0 D0\<close> \<open>x2 \<notin> D0\<close> TyV
-    using  assume_assign_non_empty by (blast dest: assume_assign_non_empty)
+     by (blast dest: assume_assign_non_empty)
   have U1Dep: "dependent A \<Lambda>' \<Omega> ?U1Normal (D0 \<union> {x2})"
     using \<open>dependent A \<Lambda>' \<Omega> U0 D0\<close> \<open>x2 \<notin> D0\<close> RedX1
     by (blast dest: assume_assign_dependent)
@@ -997,7 +1111,7 @@ next
         "\<forall>u\<in>U2.
          \<exists>su. (A,M,\<Lambda>',\<Gamma>,\<Omega> \<turnstile> \<langle>cs,Normal u\<rangle> [\<rightarrow>] su) \<and>
               (s' = Failure \<longrightarrow> su = Failure) \<and> (\<forall>ns'. s' = Normal ns' \<longrightarrow> su = Normal u \<and>
-              nstate_rel \<Lambda> \<Lambda>' (update_nstate_rel (R(x \<mapsto> Inl x2)) Q) ns' u \<and> rel_well_typed A \<Lambda> \<Omega> (update_nstate_rel (R(x \<mapsto> Inl x2)) Q) ns')"
+              nstate_rel \<Lambda> \<Lambda>' (update_nstate_rel (R(x \<mapsto> Inl x2)) Q) ns' u \<and> nstate_old_rel \<Lambda> \<Lambda>' R_old ns' u \<and> rel_well_typed A \<Lambda> \<Omega> (update_nstate_rel (R(x \<mapsto> Inl x2)) Q) ns')"
     by blast
   hence U2Sub':"U2 \<subseteq> U0" and  U2Dep':"dependent A \<Lambda>' \<Omega> U2 (D0 \<union> set (x2 # W))" and 
     RedAssume2:"\<And>u. u \<in> U2 \<Longrightarrow> A,M,\<Lambda>',\<Gamma>,\<Omega> \<turnstile> \<langle>Assume ((Var x2) \<guillemotleft>Eq\<guillemotright> (Var x1)),Normal u\<rangle> \<rightarrow> Normal u"
@@ -1005,21 +1119,71 @@ next
   show ?case
     apply (rule exI, intro conjI, rule U2Sub', rule \<open>U2 \<noteq> {}\<close>, rule U2Dep', rule ballI)
     using U2Rel RedAssume2 update_nstate_rel_cons
-    by (metis RedCmdListCons)  
+    by (metis RedCmdListCons)
+next
+  case (PSyncConst R x l W x2 Q cs)
+  hence "x2 \<notin> D0" by simp
+  let ?U1 = "(set_red_cmd A M \<Lambda>' \<Gamma> \<Omega> (Assume ((Var x2) \<guillemotleft>Eq\<guillemotright> (Lit l))) U0)"
+  let ?U1Normal = "{ns. Normal ns \<in> ?U1}"   
+  have U1Sub:"?U1Normal \<subseteq> U0"
+    by (simp add: passive_states_subset)
+  have RedLit:"\<forall>u\<in>U0. A,\<Lambda>',\<Gamma>,\<Omega> \<turnstile> \<langle>Lit l,u\<rangle> \<Down> (LitV l)"        
+    by (blast intro: RedLit)
+  from \<open>R x = Some (Inr l)\<close> \<open>rel_well_typed A \<Lambda> \<Omega> R ns\<close> obtain \<tau> where
+    "lookup_var \<Lambda> ns x = Some (LitV l)" and LookupTy:"lookup_var_ty \<Lambda> x = Some \<tau>" and 
+    TyV:"TPrim (type_of_lit l) = instantiate \<Omega> \<tau>"
+    unfolding rel_well_typed_def rel_const_correct_def by blast  
+  hence TypLit:"type_of_val A (LitV l) = instantiate \<Omega> \<tau>" by simp
+  from LookupTy have "lookup_var_ty \<Lambda>' x2 = Some \<tau>" using \<open>type_rel \<Lambda> \<Lambda>' ((x, Inl x2) # Q)\<close> 
+    unfolding type_rel_def by simp    
+  hence U1NonEmpty: "?U1Normal \<noteq> {}" using RedLit \<open>U0 \<noteq> {}\<close> \<open>dependent A \<Lambda>' \<Omega> U0 D0\<close> \<open>x2 \<notin> D0\<close> TyV
+    using  assume_assign_non_empty[OF RedLit TypLit] by blast
+  have U1Dep: "dependent A \<Lambda>' \<Omega> ?U1Normal (D0 \<union> {x2})"
+    using \<open>dependent A \<Lambda>' \<Omega> U0 D0\<close> \<open>x2 \<notin> D0\<close> RedLit
+    by (blast dest: assume_assign_dependent)
+  have RelStates: "nstate_rel_states \<Lambda> \<Lambda>' (R(x \<mapsto> Inl x2)) ns ?U1Normal" 
+    using \<open>nstate_rel_states \<Lambda> \<Lambda>' R ns U0\<close>  \<open>rel_well_typed A \<Lambda> \<Omega> R ns\<close> \<open>R x = Some (Inr l)\<close>
+    by (blast dest: assume_sync_const_nstate_rel)
+  have RelOldStates: "nstate_old_rel_states \<Lambda> \<Lambda>' R_old ns ?U1Normal" 
+    using \<open>nstate_old_rel_states \<Lambda> \<Lambda>' R_old ns U0\<close> U1Sub nstate_old_rel_states_update nstate_old_rel_states_subset
+      by blast
+  have RedAssume: "\<And>u. u \<in> ?U1Normal \<Longrightarrow> A,M,\<Lambda>',\<Gamma>,\<Omega> \<turnstile> \<langle>Assume ((Var x2) \<guillemotleft>Eq\<guillemotright> (Lit l)),Normal u\<rangle> \<rightarrow> Normal u"    
+    by (rule passive_states_propagate_2) simp
+
+  from \<open>distinct (x2 # W)\<close> \<open>set (x2 # W) \<inter> D0 = {}\<close> have "distinct W" and "set W \<inter> (D0 \<union> {x2}) = {}" by auto
+  from \<open>type_rel \<Lambda> \<Lambda>' ((x, (Inl x2)) # Q)\<close> have QTyRel:"type_rel \<Lambda> \<Lambda>' Q" by (simp add: type_rel_def)
+  from \<open>rel_well_typed A \<Lambda> \<Omega> R ns\<close> have Rel_wt:\<open>rel_well_typed A \<Lambda> \<Omega> (R(x \<mapsto> (Inl x2))) ns\<close> using \<open>R x = Some (Inr l)\<close> by (simp add: rel_well_typed_def rel_const_correct_def)
+  from PSyncConst.IH[OF \<open>A,M,\<Lambda>,\<Gamma>,\<Omega> \<turnstile> \<langle>[],Normal ns\<rangle> [\<rightarrow>] s'\<close> U1Dep RelStates RelOldStates Rel_wt \<open>set W \<inter> (D0 \<union> {x2}) = {}\<close> U1NonEmpty QTyRel \<open>distinct W\<close>]
+  obtain U2 where 
+      U2Sub:"U2 \<subseteq> ?U1Normal" and
+      "U2 \<noteq> {}" and U2Dep:"dependent A \<Lambda>' \<Omega> U2 (D0 \<union> {x2} \<union> set W)" and
+      U2Rel:
+        "\<forall>u\<in>U2.
+         \<exists>su. (A,M,\<Lambda>',\<Gamma>,\<Omega> \<turnstile> \<langle>cs,Normal u\<rangle> [\<rightarrow>] su) \<and>
+              (s' = Failure \<longrightarrow> su = Failure) \<and> (\<forall>ns'. s' = Normal ns' \<longrightarrow> su = Normal u \<and>
+              nstate_rel \<Lambda> \<Lambda>' (update_nstate_rel (R(x \<mapsto> Inl x2)) Q) ns' u \<and> nstate_old_rel \<Lambda> \<Lambda>' R_old ns' u \<and> rel_well_typed A \<Lambda> \<Omega> (update_nstate_rel (R(x \<mapsto> Inl x2)) Q) ns')"
+    by blast
+   hence U2Sub':"U2 \<subseteq> U0" and  U2Dep':"dependent A \<Lambda>' \<Omega> U2 (D0 \<union> set (x2 # W))" and 
+    RedAssume2:"\<And>u. u \<in> U2 \<Longrightarrow> A,M,\<Lambda>',\<Gamma>,\<Omega> \<turnstile> \<langle>Assume ((Var x2) \<guillemotleft>Eq\<guillemotright> (Lit l)),Normal u\<rangle> \<rightarrow> Normal u"
+      using U1Sub RedAssume by auto
+  show ?case
+    apply (rule exI, intro conjI, rule U2Sub', rule \<open>U2 \<noteq> {}\<close>, rule U2Dep', rule ballI)
+    using U2Rel RedAssume2 update_nstate_rel_cons
+    by (metis RedCmdListCons)
 next
   case (PNil R)
-  then show ?case
-    by (metis RedCmdListNil empty_set nstate_rel_states_def state.distinct(1) state.inject step_nil_same subset_refl sup_bot.right_neutral update_nstate_rel_nil) 
+  thus ?case
+  by (metis RedCmdListNil empty_set nstate_rel_states_def nstate_old_rel_states_def state.distinct(1) state.inject step_nil_same subset_refl sup_bot.right_neutral update_nstate_rel_nil)
 qed
 
 definition passive_block_conclusion
-  where "passive_block_conclusion A M \<Lambda> \<Lambda>' \<Gamma> \<Omega> U0 D1 R cs2 s' = 
-  (\<exists> U1 \<subseteq> U0. U1 \<noteq> {} \<and> dependent A \<Lambda>' \<Omega> U1 D1 \<and> passive_sim A M \<Lambda> \<Lambda>' \<Gamma> \<Omega> cs2 s' R U1)"
+  where "passive_block_conclusion A M \<Lambda> \<Lambda>' \<Gamma> \<Omega> U0 D1 R R_old cs2 s' = 
+  (\<exists> U1 \<subseteq> U0. U1 \<noteq> {} \<and> dependent A \<Lambda>' \<Omega> U1 D1 \<and> passive_sim A M \<Lambda> \<Lambda>' \<Gamma> \<Omega> cs2 s' R R_old U1)"
 
 definition passive_lemma_assms :: "'a absval_ty_fun \<Rightarrow> method_context \<Rightarrow> var_context \<Rightarrow> var_context \<Rightarrow> 
                    'a fun_interp \<Rightarrow> rtype_env \<Rightarrow> vname list \<Rightarrow> passive_rel \<Rightarrow> passive_rel \<Rightarrow> 
-                  ('a nstate) set \<Rightarrow> vname set \<Rightarrow> cmd list \<Rightarrow> 'a nstate \<Rightarrow> bool"
-  where "passive_lemma_assms A M \<Lambda> \<Lambda>' \<Gamma> \<Omega> W R R_old U0 D0 cs1 ns = 
+                  ('a nstate) set \<Rightarrow> vname set \<Rightarrow> 'a nstate \<Rightarrow> bool"
+  where "passive_lemma_assms A M \<Lambda> \<Lambda>' \<Gamma> \<Omega> W R R_old U0 D0 ns = 
           (nstate_rel_states \<Lambda> \<Lambda>' R ns U0 \<and> 
            nstate_old_rel_states \<Lambda> \<Lambda>' R_old ns U0 \<and>
           rel_well_typed A \<Lambda> \<Omega> R ns \<and>
@@ -1029,16 +1193,17 @@ definition passive_lemma_assms :: "'a absval_ty_fun \<Rightarrow> method_context
 lemma passification_block_lemma_compact:
   assumes 
           "A,M,\<Lambda>,\<Gamma>,\<Omega> \<turnstile> \<langle>cs1, Normal ns\<rangle> [\<rightarrow>] s'"
-          "passive_lemma_assms A M \<Lambda> \<Lambda>' \<Gamma> \<Omega> W R R_old U0 D0 cs1 ns" and
+          "passive_lemma_assms A M \<Lambda> \<Lambda>' \<Gamma> \<Omega> W R R_old U0 D0 ns" and
           "passive_cmds_rel (snd \<Lambda>) R_old W R Q cs1 cs2" and
           "type_rel \<Lambda> \<Lambda>' Q" and
           "distinct W"
-  shows "passive_block_conclusion A M \<Lambda> \<Lambda>' \<Gamma> \<Omega> U0 (D0 \<union> (set W)) (update_nstate_rel R Q) cs2 s'"
+  shows "passive_block_conclusion A M \<Lambda> \<Lambda>' \<Gamma> \<Omega> U0 (D0 \<union> (set W)) (update_nstate_rel R Q) R_old cs2 s'"
   using assms
   unfolding passive_lemma_assms_def passive_block_conclusion_def
   using passification_block_lemma_aux by meson
 
 text \<open>CFG proofs\<close>
+
 definition passive_cfg_assms
   where "passive_cfg_assms A M \<Lambda> \<Lambda>' \<Gamma> \<Omega> G W R U0 D0 m m' ns s' = 
           ( (A,M,\<Lambda>,\<Gamma>,\<Omega>,G \<turnstile> (m, Normal ns) -n\<rightarrow>* (m',s')) \<and>
@@ -1051,6 +1216,79 @@ definition passive_sim_cfg
               (\<forall>u \<in> U. \<exists> m_p' su. (A,M,\<Lambda>',\<Gamma>,\<Omega>, G \<turnstile> (m_p, Normal u) -n\<rightarrow>* (m_p',su)) \<and> 
                        (s' = Failure \<longrightarrow> su = Failure))"
 
+definition passive_sim_cfg_fail
+  where "passive_sim_cfg_fail A M \<Lambda>' \<Gamma> \<Omega> G u m_p \<equiv> 
+              (\<exists> m_p'. (A,M,\<Lambda>',\<Gamma>,\<Omega>, G \<turnstile> (m_p, Normal u) -n\<rightarrow>* (m_p', Failure)))"
+
+lemma final_rel_lemma:
+  assumes "A,M,\<Lambda>1,\<Gamma>,\<Omega>,G \<turnstile> (m, Normal ns) -n\<rightarrow>* (m',s')" and
+          "nstate_rel_states \<Lambda>1 \<Lambda>2 R ns U0" and
+          "rel_well_typed A \<Lambda>1 \<Omega> R ns" and
+          "dependent A \<Lambda>2 \<Omega> U0 D0" and
+          "(set W) \<inter> D0 = {}" and
+          "U0 \<noteq> {}"
+  shows "\<exists> U1 \<subseteq> U0. U1 \<noteq> {} \<and> dependent A \<Lambda>2 \<Omega> U1 D1 \<and> passive_sim_cfg A M \<Lambda>2 \<Gamma> \<Omega> G' U1 (Inl 4) s'"
+  oops
+
+(*
+lemma red_cfg_multi_backwards_step:
+  assumes
+   Red: "A,M,\<Lambda>,\<Gamma>,\<Omega>,G \<turnstile> (Inl m, (Normal  n_s)) -n\<rightarrow>* (m', s')" and
+   Block: "node_to_block G ! m = cs" and
+   BlockCorrect: "\<And> s''. A,M,\<Lambda>,\<Gamma>,\<Omega> \<turnstile> \<langle>cs, Normal n_s\<rangle> [\<rightarrow>] s'' \<Longrightarrow> 
+            s'' \<noteq> Failure \<and> (\<forall>  n_s'. ((s'' = (Normal  n_s')) \<longrightarrow> (n_s' = n_s) \<and> vcsuc))" and
+   SuccCorrect:"\<And> msuc s2 m2. List.member (out_edges(G) ! m) msuc \<Longrightarrow> A,M,\<Lambda>,\<Gamma>,\<Omega>,G \<turnstile> (Inl(msuc), Normal n_s) -n\<rightarrow>* (m2, s2) \<Longrightarrow> vcsuc \<Longrightarrow> s2 \<noteq> Failure"*)
+
+definition dependent_2
+  where "dependent_2 A \<Lambda>' \<Omega> U0 m = dependent A \<Lambda>' \<Omega> U0 {y. y \<le> m}"
+
+definition passive_lemma_assms_2 :: "'a absval_ty_fun \<Rightarrow> method_context \<Rightarrow> var_context \<Rightarrow> var_context \<Rightarrow> 
+                   'a fun_interp \<Rightarrow> rtype_env \<Rightarrow> vname \<Rightarrow> passive_rel \<Rightarrow> passive_rel \<Rightarrow> 
+                  ('a nstate) set \<Rightarrow> vname set \<Rightarrow> 'a nstate \<Rightarrow> bool"
+  where "passive_lemma_assms_2 A M \<Lambda> \<Lambda>' \<Gamma> \<Omega> w_min R R_old U0 D0 ns = 
+          (nstate_rel_states \<Lambda> \<Lambda>' R ns U0 \<and> 
+           nstate_old_rel_states \<Lambda> \<Lambda>' R_old ns U0 \<and>
+          rel_well_typed A \<Lambda> \<Omega> R ns \<and>
+          dependent A \<Lambda>' \<Omega> U0 D0 \<and> {w. w \<ge> w_min} \<inter> D0 = {} \<and>
+          U0 \<noteq> {})"
+
+lemma passive_assms_convert: 
+  assumes "passive_lemma_assms_2 A M \<Lambda> \<Lambda>' \<Gamma> \<Omega> w_min R R_old U0 D0 ns" and 
+          "W \<noteq> [] \<Longrightarrow> w_min \<le> Min (set W)"
+        shows "passive_lemma_assms A M \<Lambda> \<Lambda>' \<Gamma> \<Omega> W R R_old U0 D0 ns"
+  using assms
+  unfolding passive_lemma_assms_2_def passive_lemma_assms_def
+  by force
+
+lemma passive_assms_convert_2: 
+  assumes "passive_lemma_assms A M \<Lambda> \<Lambda>' \<Gamma> \<Omega> W R R_old U0 D0 ns" and 
+          "Max (set W) < w_min" and
+          "D0 \<inter> {w. w \<ge> w_min} = {}"
+  shows "passive_lemma_assms_2 A M \<Lambda> \<Lambda>' \<Gamma> \<Omega> w_min R R_old U0 D0 ns"
+  using assms
+  unfolding passive_lemma_assms_2_def passive_lemma_assms_def
+  by (simp add: inf_commute)
+
+lemma passive_assms_2_ext:
+  assumes "passive_lemma_assms_2 A M \<Lambda> \<Lambda>' \<Gamma> \<Omega> w_min R R_old U0 D0 ns" and 
+          "w_min \<le> w'"
+  shows "passive_lemma_assms_2 A M \<Lambda> \<Lambda>' \<Gamma> \<Omega> w' R R_old U0 D0 ns"
+  using assms
+  unfolding passive_lemma_assms_2_def 
+  using order.trans by fastforce
+
+
+lemma passification_cfg_lemma:
+  assumes "A,M,\<Lambda>,\<Gamma>,\<Omega>,G \<turnstile> ((Inl m), Normal ns) -n\<rightarrow>* (m',s')" and
+          "nstate_rel_states \<Lambda> \<Lambda>' R ns U0" and
+          "rel_well_typed A \<Lambda> \<Omega> R ns" and
+          "dependent A \<Lambda>' \<Omega> U0 D0" and
+          "(set W) \<inter> D0 = {}" and
+          "U0 \<noteq> {}" and
+          "\<And> msuc s2 m2. List.member (out_edges(G) ! m) msuc \<Longrightarrow> 
+                    \<exists>m_suc_pas. \<exists> U2 \<subseteq> U0. U2 \<noteq> {} \<and> passive_sim_cfg A M \<Lambda>2 \<Gamma> \<Omega> G_passive U2 m_suc_pas s' "
+        shows "\<exists> U1 \<subseteq> U0. U1 \<noteq> {} \<and> passive_sim_cfg A M \<Lambda>2 \<Gamma> \<Omega> G_passive U1 m_passive s'"
+  oops
 (*
 definition passive_cfg_conclusion
   where "passive_cfg_conclusion A M \<Lambda> \<Lambda>' \<Gamma> \<Omega> G U0 D1 R m m' s' = 
@@ -1062,8 +1300,129 @@ definition passive_cfg_lemma
            passive_cfg_conclusion A M \<Lambda> \<Lambda>' \<Gamma> \<Omega> G U0 (D0 \<union> (set W)) R m_p m_p' s')"
 *)
 
+lemma set_helper: 
+  assumes "(w1 :: nat) \<le> w2"
+  shows "{w. w \<ge> w2} \<subseteq> {w. w \<ge> w1}"
+  using assms
+  by auto
+
+lemma set_helper_2:
+  assumes "W \<noteq> []"
+  shows "{w::nat. w \<ge> (Max (set W))+1} \<inter> (set W) = {}"
+proof (rule, rule)
+  fix x
+  assume "x \<in> {w. Max (set W) + 1 \<le> w} \<inter> set W"
+  hence  Elem1:"x \<in> {w. Max (set W) + 1 \<le> w}" and "x \<in> (set W)" by auto
+  from \<open>x \<in> (set W)\<close> \<open>W \<noteq> []\<close> have "x \<le> Max (set W)" by force
+  thus "x \<in> {}" using Elem1 by simp
+next
+  show "{} \<subseteq> {w. Max (set W) + 1 \<le> w} \<inter> set W" by simp
+qed
   
-          
-          
+lemma passification_cfg_helper:
+  assumes 
+   "A,M,\<Lambda>1,\<Gamma>,\<Omega>,G1 \<turnstile> ((Inl m), Normal ns) -n\<rightarrow>* (m',s')" and
+   SameEdges:"out_edges G1 = out_edges G2" and (* requiring that G1 and G2 have the same edges makes the successor assumption easier *)
+   PassiveAssms: "passive_lemma_assms_2 A M \<Lambda>1 \<Lambda>2 \<Gamma> \<Omega> w_min R R_old U0 D0 ns" and
+   Block: "node_to_block G1 ! m = cs" and
+   BlockPassive: "node_to_block G2 ! m = cs2" and
+   BlockCorrect: "\<And> s''. A,M,\<Lambda>1,\<Gamma>,\<Omega> \<turnstile> \<langle>cs,Normal ns\<rangle> [\<rightarrow>] s'' \<Longrightarrow>
+                  passive_lemma_assms A M \<Lambda>1 \<Lambda>2 \<Gamma> \<Omega> W R R_old U0 D0 ns \<Longrightarrow>                  
+                  passive_block_conclusion A M \<Lambda>1 \<Lambda>2 \<Gamma> \<Omega> U0 (D0 \<union> (set W)) (update_nstate_rel R Q) R_old cs2 s''" and
+   BlockFree: "W \<noteq> [] \<Longrightarrow> w_min \<le> Min (set W)" and 
+   MaxAssm: "W \<noteq> [] \<Longrightarrow> w_max_suc = 1+Max (set W)" and
+   MinSmallerMax: "w_min < w_max_suc" and
+   SuccCorrect:
+             "\<And> U0 D0 msuc s' ns'. List.member (out_edges(G1) ! m) msuc \<Longrightarrow>
+                    A,M,\<Lambda>1,\<Gamma>,\<Omega>,G1 \<turnstile> ((Inl msuc), Normal ns') -n\<rightarrow>* (m',s') \<Longrightarrow>  
+                    passive_lemma_assms_2 A M \<Lambda>1 \<Lambda>2 \<Gamma> \<Omega> w_max_suc (update_nstate_rel R Q) R_old U0 D0 ns' \<Longrightarrow>
+                    s' = Failure \<longrightarrow> (\<exists> u \<in> U0. passive_sim_cfg_fail A M \<Lambda>2 \<Gamma> \<Omega> G2 u (Inl msuc))"
+           shows "s' = Failure \<longrightarrow> (\<exists> u \<in> U0. passive_sim_cfg_fail A M \<Lambda>2 \<Gamma> \<Omega> G2 u (Inl m))"
+proof (cases rule: converse_rtranclpE2[OF assms(1)])
+  case 1
+  then show ?thesis by auto
+next
+  case (2 a b)
+  then show ?thesis 
+  proof cases
+    case (RedNormalSucc csTemp ns' n')
+     let ?R' = "update_nstate_rel R Q"
+    let ?D1 = "D0 \<union> (set W)"
+    from RedNormalSucc have "csTemp = cs" using Block by simp
+    with RedNormalSucc BlockCorrect  have "passive_block_conclusion A M \<Lambda>1 \<Lambda>2 \<Gamma> \<Omega> U0 ?D1 ?R' R_old cs2 (Normal ns')"
+      using passive_assms_convert[OF PassiveAssms BlockFree]
+      by blast
+    from this obtain U1 where "U1 \<subseteq> U0" and"U1 \<noteq> {}" and DepU1:"dependent A \<Lambda>2 \<Omega> U1 ?D1" and SimU1:"passive_sim A M \<Lambda>1 \<Lambda>2 \<Gamma> \<Omega> cs2 (Normal ns') ?R' R_old U1"
+      unfolding passive_block_conclusion_def by blast     
+    from PassiveAssms have "D0 \<inter> {w. w \<ge> w_min} = {}" unfolding passive_lemma_assms_2_def by blast   
+    hence "D0 \<inter> {w. w \<ge> w_max_suc} = {}" using MaxAssm BlockFree set_helper MinSmallerMax by force
+    moreover have "W \<noteq> [] \<Longrightarrow> (set W) \<inter> {w. w \<ge> w_max_suc} = {}" using MaxAssm set_helper_2 
+      by (simp add: Int_commute)
+    ultimately have Disj:"(D0 \<union> (set W)) \<inter> {w. w \<ge> w_max_suc} = {}"
+      by (cases "W = []") auto      
+    have SucResult:"s' = Failure \<longrightarrow> (\<exists>u\<in>U1. passive_sim_cfg_fail A M \<Lambda>2 \<Gamma> \<Omega> G2 u (Inl n'))"  
+      apply (rule SuccCorrect)
+        apply (simp add: RedNormalSucc)
+      using RedNormalSucc 2 apply fastforce
+      unfolding passive_lemma_assms_2_def
+      apply (intro conjI)
+      using SimU1 apply (simp add: passive_sim_def nstate_rel_states_def)
+      using SimU1 apply (simp add:  passive_sim_def nstate_old_rel_states_def)
+      using SimU1 \<open>U1 \<noteq> {}\<close> apply (simp add: passive_sim_def) apply blast
+      apply (rule DepU1)
+      using Disj  apply (simp add: inf_commute) 
+      apply (rule \<open>U1 \<noteq> {}\<close>)
+      done
+    show ?thesis
+    proof 
+      assume "s' = Failure"
+      with SucResult obtain u m_p' where "u \<in> U1" and RedPassiveRemaining:"(A,M,\<Lambda>2,\<Gamma>,\<Omega>, G2 \<turnstile> ((Inl n'), Normal u) -n\<rightarrow>* (m_p', Failure))"
+        unfolding passive_sim_cfg_fail_def using \<open>U1 \<subseteq> U0\<close> by auto
+      hence "u \<in> U0" using \<open>U1 \<subseteq> U0\<close> by auto
+      (* simulation of passive block *)
+      from SimU1 have RedCs2:" A,M,\<Lambda>2,\<Gamma>,\<Omega> \<turnstile> \<langle>cs2,Normal u\<rangle> [\<rightarrow>] Normal u" unfolding passive_sim_def using \<open>u \<in> U1\<close>
+        by simp
+      
+      show "\<exists>u\<in>U0. passive_sim_cfg_fail A M \<Lambda>2 \<Gamma> \<Omega> G2 u (Inl m)"
+       apply (rule bexI[OF _ \<open>u \<in> U0\<close>], (unfold passive_sim_cfg_fail_def), rule exI[where ?x=m_p'])
+        apply (rule converse_rtranclp_into_rtranclp)
+         apply (rule red_cfg.RedNormalSucc)
+           apply (rule BlockPassive)
+          apply (rule RedCs2)
+        using \<open>List.member (out_edges G1 ! m) n'\<close> SameEdges apply simp
+        apply (rule RedPassiveRemaining)
+        done
+    qed
+  next
+    case (RedNormalReturn cs ns')
+    with \<open>A,M,\<Lambda>1,\<Gamma>,\<Omega>,G1 \<turnstile>(a, b) -n\<rightarrow>* (m', s')\<close> have "s' = Normal ns'" using finished_remains 
+      by blast
+    thus ?thesis by simp
+  next
+    case (RedFailure csTemp)
+    let ?R' = "update_nstate_rel R Q"
+    let ?D1 = "D0 \<union> (set W)"
+    from RedFailure have "csTemp = cs" using Block by simp
+    with RedFailure BlockCorrect have "passive_block_conclusion A M \<Lambda>1 \<Lambda>2 \<Gamma> \<Omega> U0 ?D1 ?R' R_old cs2 Failure"
+      using passive_assms_convert[OF PassiveAssms BlockFree] by simp
+    from this obtain U1 where "U1 \<subseteq> U0" and "U1 \<noteq> {}" and  SimU1:"passive_sim A M \<Lambda>1 \<Lambda>2 \<Gamma> \<Omega> cs2 Failure ?R' R_old U1"
+      unfolding passive_block_conclusion_def by blast
+    from this obtain u where "u \<in> U0" and RedCs2:"A,M,\<Lambda>2,\<Gamma>,\<Omega> \<turnstile> \<langle>cs2, Normal u\<rangle> [\<rightarrow>] Failure" unfolding passive_sim_def by blast
+    show ?thesis 
+      apply (rule impI)
+      apply (rule bexI[OF _ \<open>u \<in> U0\<close>])
+      unfolding passive_sim_cfg_fail_def
+      apply (rule exI[where ?x="Inr ()"])
+      apply (rule converse_rtranclp_into_rtranclp)
+       apply (rule red_cfg.RedFailure)
+        apply (rule BlockPassive)
+       apply (rule RedCs2)
+      apply (blast dest: finished_remains)
+      done
+  next
+    case (RedMagic cs)
+    then show ?thesis using finished_remains 2 by blast
+  qed
+qed                   
 
 end
